theories/FMset/FMsetTC.v
@@ -1,0 +1,66 @@
+(* 
+  Autor(s):
+    Andrej Dudenhefner (1) 
+  Affiliation(s):
+    (1) Saarland Informatics Campus, Saarland University, Saarbrücken, Germany
+*)
+
+(* 
+  Problem:
+    Finite multiset term constraint solvability (FMsetTC)
+
+  Finite multisets with one constant 0 and one unary constructor h
+  A finite multiset A is represented by a list of its elements.
+  The element (h^n 0) is represented by the natural number n.
+
+  Terms t, u:
+    t, u ::= zero | t ⊍ u | h (t) | x : nat
+    where x ranges over multiset variables
+  
+  Constraints:
+    t ≐ u 
+
+  Term Interpretation:
+    φ(zero) = [0]
+    φ(t ⊍ u) = φ(t) ++ φ(u)
+    φ(h (t)) = map h (φ(t))
+
+  FMsetTC:
+    Given a list (t₁ ≐ u₁),...,(tₙ ≐ uₙ) of constraints,
+    is there a valuation φ : nat -> list nat such that
+    φ(t₁) ≡ φ(u₁),..., φ(tₙ) ≡ φ(uₙ),
+    where ≡ is equality up to permutation?
+  
+  References:
+    [1] Paliath Narendran: Solving Linear Equations over Polynomial Semirings.
+      LICS 1996: 466-472, doi: 10.1109/LICS.1996.561463
+*)
+
+Require Import PeanoNat.
+Require Import List.
+Import ListNotations.
+
+From Undecidability Require Import Problems.FMsetC.
+
+(* terms *)
+Inductive mset_term : Set :=
+  | mset_term_zero : mset_term
+  | mset_term_var : nat -> mset_term
+  | mset_term_plus : mset_term -> mset_term -> mset_term
+  | mset_term_h : mset_term -> mset_term.
+
+(* evaluate an mset wrt. a valuation φ *)
+Fixpoint mset_sem (φ : nat -> list nat) (A : mset_term) : list nat :=
+  match A with
+    | mset_term_zero => [0]
+    | mset_term_var x => φ x
+    | mset_term_plus A B => (mset_sem φ A) ++ (mset_sem φ B)
+    | mset_term_h A => map S (mset_sem φ A)
+  end.
+
+(* list of constraints *)
+Definition FMsetTC_PROBLEM := list (mset_term * mset_term).
+
+(* is there a valuation φ that satisfies all contraints *)
+Definition FMsetTC_SAT (l : FMsetTC_PROBLEM) := 
+  exists (φ : nat -> list nat), forall (A B : mset_term), In (A, B) l -> (mset_sem φ A) ≡ (mset_sem φ B).
