theories/FMset/mset_eq_utils.v
@@ -1,0 +1,176 @@
+(* 
+  Autor(s):
+    Andrej Dudenhefner (1) 
+  Affiliation(s):
+    (1) Saarland Informatics Campus, Saarland University, Saarbrücken, Germany
+*)
+
+Require Import ssreflect ssrbool ssrfun.
+Require Import PeanoNat Psatz.
+Require Import List.
+Import ListNotations.
+
+From Undecidability Require Import Problems.FMsetC.
+From Undecidability Require Import FMset.mset_utils.
+
+Arguments mset_eq !A !B.
+
+(* eq facts *)
+Lemma eq_refl {A} : A ≡ A.
+Proof. done. Qed.
+
+Lemma eq_eq {A B}: A = B -> A ≡ B.
+Proof. by move=> ->. Qed.
+  
+Lemma eq_symm {A B} : A ≡ B -> B ≡ A.
+Proof. by firstorder done. Qed.
+  
+Lemma eq_in_iff {A B} : A ≡ B -> forall c, In c A <-> In c B.
+Proof.
+  rewrite /mset_eq => H c. constructor=> Hc.
+  - have := iffLR (count_occ_In Nat.eq_dec A c) Hc.
+    move: (H c) => ->.
+    by move /(count_occ_In Nat.eq_dec B c).
+  - have := iffLR (count_occ_In Nat.eq_dec B c) Hc.
+    move: (H c) => <-.
+    by move /(count_occ_In Nat.eq_dec A c).
+Qed.
+
+Lemma eq_nilE {A} : [] ≡ A -> A = [].
+Proof.
+  case: A.
+    done.
+  move=> a A /eq_in_iff /(_ a) /iffRL. apply: unnest.
+    by left.
+  done.
+Qed.
+
+Lemma eq_trans {A B C} : A ≡ B -> B ≡ C -> A ≡ C.
+Proof.
+  rewrite /mset_eq => + + c.
+  move=> /(_ c) + /(_ c).
+  by move=> -> ->.
+Qed.
+
+Lemma eq_Forall_iff {A B} : A ≡ B -> forall P, (Forall P A <-> Forall P B).
+Proof.
+  move /eq_in_iff => H P.
+  rewrite ? Forall_forall. constructor; by firstorder done.
+Qed.
+
+Lemma eq_lr {A B A' B'}:
+  A ≡ A' -> B ≡ B' -> (A ≡ B) <-> (A' ≡ B').
+Proof.
+  move=> HA HB. constructor.
+  - move /eq_trans. move /(_ _ HB). 
+    move /(eq_trans _). by move /(_ _ (eq_symm HA)). 
+  - move /eq_trans. move /(_ _ (eq_symm HB)). 
+    move /(eq_trans _). by move /(_ _ HA).
+Qed. 
+
+Lemma eq_appI {A B A' B'} : A ≡ A' -> B ≡ B' -> A ++ B ≡ A' ++ B'.
+Proof.
+  rewrite /mset_eq => + + c. move=> /(_ c) + /(_ c).
+  rewrite ? count_occ_app. by move=> -> ->.
+Qed.
+
+(* solves trivial multiset equalities *)
+Ltac eq_trivial := 
+  move=> ?; rewrite ? (count_occ_app, count_occ_cons, count_occ_nil); unlock; by lia.
+    
+Lemma eq_cons_iff {a A B} : (a :: A) ≡ (a :: B) <-> A ≡ B.
+Proof.
+  rewrite /mset_eq. constructor.
+  all: move=> H c; move: {H}(H c); rewrite ? count_occ_cons ? in_cons_iff; unlock.
+  all: by rewrite Nat.add_cancel_l.
+Qed.
+
+Lemma eq_app_iff {A B C} : (A ++ B) ≡ (A ++ C) <-> B ≡ C.
+Proof.
+  elim: A.
+    done.
+  move=> a A IH /=.
+  by rewrite eq_cons_iff.
+Qed.
+
+Lemma eq_length {A B} : A ≡ B -> length A = length B.
+  elim /(measure_ind (@length nat)) : A B.
+  case.
+    by move=> _ B /eq_nilE ->.
+  move=> a A IH B /copy [/eq_in_iff /(_ a) /iffLR]. apply: unnest.
+    by left.
+  move /(@in_split _ _) => [B1 [B2 ->]].
+  under (eq_lr eq_refl (B' := a :: (B1 ++ B2))).
+    by eq_trivial.
+  move /eq_cons_iff. move /IH. apply: unnest.
+    done.
+  rewrite ? app_length => /=. by lia.
+Qed.
+
+Lemma eq_repeatE {a A n} : repeat a n ≡ A -> A = repeat a n.
+Proof.
+  move=> /copy [/eq_length]. rewrite repeat_length => HlA.
+  move /eq_Forall_iff /(_ (fun c => a = c)) /iffLR. apply: unnest.
+    clear. elim: n.
+      by constructor.
+    firstorder (by constructor).
+  subst n.
+  elim: A.
+    done.
+  move=> b A IH /Forall_cons_iff [<-] /IH -> /=.
+  by rewrite repeat_length.
+Qed.
+
+Lemma eq_singletonE {a A} : [a] ≡ A -> A = [a].
+Proof.
+  have -> : [a] = repeat a 1 by done.
+  by move /eq_repeatE.
+Qed.
+
+Lemma eq_mapE {A} : map S A ≡ A -> A = [].
+Proof.
+  case (nil_or_ex_max A).
+    done.
+  move=> [a [Ha /Forall_forall HA]] /eq_in_iff /(_ (S a)) /iffLR.
+  rewrite in_map_iff. apply: unnest.
+    by exists a.
+  move /HA. by lia.
+Qed.
+
+Lemma eq_consP {a A B}: a :: A ≡ a :: B <-> A ≡ B.
+Proof.
+  rewrite /mset_eq. constructor; move=> + c => /(_ c).
+  all: rewrite ? count_occ_cons; by lia.
+Qed.
+
+Lemma eq_consE {a A B}: a :: A ≡ B -> exists B1 B2, B = B1 ++ (a :: B2) /\ A ≡ (B1 ++ B2).
+Proof.
+  move=> /copy [/mset_eq_utils.eq_in_iff /(_ a) /iffLR /(_ ltac:(by left))].
+  move /(@in_split _ _) => [B1 [B2 ->]].
+  under (mset_eq_utils.eq_lr mset_eq_utils.eq_refl (B' := a :: (B1 ++ B2))).
+    by mset_eq_utils.eq_trivial.
+  move /mset_eq_utils.eq_consP => H.
+  exists B1, B2. by constructor.
+Qed.
+
+Lemma eq_app_nil_nilP {A B} : A ≡ A ++ B -> B = [].
+Proof.
+  elim: A.
+    by move /eq_nilE.
+  move=> a A IH /=.
+  by move /eq_consP.
+Qed.
+
+Lemma eq_mapI {A B} : A ≡ B -> map S A ≡ map S B.
+Proof.
+  rewrite /mset_eq => + c. move=> /(_ (Nat.pred c)).
+  case: c.
+    move=> _. 
+    have H := iffLR (count_occ_not_In _ _ _).
+    rewrite ? {}H; first last.
+      done.
+    1-2: by rewrite in_map_iff=> [[? [? ?]]].
+  move=> c. rewrite - ? (count_occ_map S Nat.eq_dec Nat.eq_dec); first last.
+    done.
+  all: move=> >; by case.
+Qed.
