theories/FMset/mset_term_utils.v
@@ -1,0 +1,29 @@
+(* 
+  Autor(s):
+    Andrej Dudenhefner (1) 
+  Affiliation(s):
+    (1) Saarland Informatics Campus, Saarland University, Saarbrücken, Germany
+*)
+
+Require Import ssreflect ssrbool ssrfun.
+Require Import List.
+Import ListNotations.
+
+From Undecidability Require Import Problems.FMsetC.
+From Undecidability Require Import FMset.FMsetTC FMset.mset_utils.
+
+Notation "t ⊍ u" := (mset_term_plus t u) (at level 40).
+Notation "'h' t" := (mset_term_h t) (at level 38).
+Notation "•0" := mset_term_zero.
+
+Coercion mset_term_var : nat >-> mset_term.
+
+Definition mset_sat (φ : nat -> list nat) (l : FMsetTC_PROBLEM) := 
+  Forall (fun '(A, B) => (mset_sem φ A) ≡ (mset_sem φ B)) l.
+
+Lemma mset_satP {φ l} : mset_sat φ l <-> (forall (A B : mset_term), In (A, B) l -> (mset_sem φ A) ≡ (mset_sem φ B)).
+Proof.
+  rewrite /mset_sat Forall_forall. constructor.
+  - move=> H A B. apply /H.
+  - move=> H [A B]. apply /H.
+Qed.
