theories/Problems/LPolyNC.v
@@ -1,0 +1,74 @@
+(* 
+  Autor(s):
+    Andrej Dudenhefner (1) 
+  Affiliation(s):
+    (1) Saarland Informatics Campus, Saarland University, Saarbrücken, Germany
+*)
+
+(* 
+  Problem:
+    Linear Polynomial[N] constraint solvability (LPolyNC)
+
+  A lineat polynomial constraint has one of the following shapes
+    x ≐ 1
+    x ≐ y + z
+    x ≐ p * y (where p is a polynomial over N)
+
+  A polynomial is mechanized by a list of its coefficients.
+
+  LPolyNC:
+    Given a list of constraints,
+    is there a valuation φ : nat -> list nat such that
+    for each constraint c we have
+      if c is x ≐ 1, then φ(x) ≃ [1]
+      if c is x ≐ y + z, then φ(x) ≃ poly_add (φ(y)) (φ(z))
+      if c is x ≐ p * y, then φ(x) ≃ poly_mult p (φ(y))
+    where ≃ is equality up to trailing zeroes?
+*)
+
+Require Import List.
+Import ListNotations.
+
+
+Definition poly : Set := list nat.
+
+(* constraint representation *)
+Inductive polyc : Set :=
+  | polyc_one : nat -> polyc
+  | polyc_sum : nat -> nat -> nat -> polyc
+  | polyc_prod : nat -> poly -> nat -> polyc.
+
+(* test whether all coefficients are equal, default to 0 *)
+Definition poly_eq (p q: poly) : Prop :=
+  forall i, nth i p 0 = nth i q 0.
+
+Notation "p ≃ q" := (poly_eq p q) (at level 65).
+
+(* polynomial addition *)
+Fixpoint poly_add (p q: poly) : poly :=
+  match p, q with
+  | [], q => q
+  | p, [] => p
+  | (c :: p), (d :: q) => (c + d) :: poly_add p q
+  end.
+
+(* polynomial multiplication *)
+Fixpoint poly_mult (p q: poly) : poly :=
+  match p with
+  | [] => []
+  | (c :: p) => poly_add (map (fun a => c * a) q) (0 :: (poly_mult p q))
+  end.
+
+Definition polyc_sem (φ: nat -> poly) (c: polyc) :=
+  match c with
+    | polyc_one x => φ x ≃ [1]
+    | polyc_sum x y z => φ x ≃ poly_add (φ y) (φ z)
+    | polyc_prod x p y => φ x ≃ poly_mult p (φ y)
+  end.
+
+(* list of constraints *)
+Definition LPolyNC_PROBLEM := list polyc.
+
+(* given a list l of constraints, 
+  is there a valuation φ satisfying each constraint? *)
+Definition LPolyNC_SAT (l : LPolyNC_PROBLEM) := exists φ, forall c, In c l -> polyc_sem φ c.
